Support SystemVerilog xor gate

cava/Cava.v
@@ -46,6 +46,7 @@ Class Cava m t `{Monad m} := {
   nand_gate : list t -> m t; (* Corresponds to the SystemVerilog primitive gate 'nand' *)
   or_gate : list t -> m t; (* Corresponds to the SystemVerilog primitive gate 'or' *)
   nor_gate : list t -> m t; (* Corresponds to the SystemVerilog primitive gate 'nor' *)
+  xor_gate : list t -> m t; (* Corresponds to the SystemVerilog primitive gate 'xor' *)
 }.
 
 Record Instance : Type := mkInstance {
@@ -105,12 +106,21 @@ Definition norNet (i : list Z) : State CavaState Z :=
          return_ o
   end.
 
+Definition xorNet (i : list Z) : State CavaState Z :=
+  cs <- get;
+  match cs with
+  | mkCavaState name o insts inputs outputs
+      => put (mkCavaState name (o+1) (cons (mkInstance "xor" o (cons o i)) insts) inputs outputs) ;;
+         return_ o
+  end.
+
 Instance CavaNet : Cava (State CavaState) Z :=
   { not_gate := notNet;
     and_gate := andNet;
     nand_gate := nandNet;
     or_gate := orNet;
     nor_gate := norNet;
+    xor_gate := xorNet;
 }.
 
 Definition setModuleNameNet (name : string) : State CavaState unit :=
@@ -165,6 +175,9 @@ Definition orBool (i : list bool) : State unit bool :=
 Definition norBool (i : list bool) : State unit bool :=
   return_ (fold_left (fun a b =>  negb (a || b)) i true).
 
+Definition xorBool (i : list bool) : State unit bool :=
+  return_ (fold_left (fun a b => xorb a b) i true).
+
 Definition inputBool (name : string) : State unit bool :=
   return_ false.
 
@@ -177,6 +190,7 @@ Instance CavaBool : Cava (State unit) bool :=
     nand_gate := nandBool;
     or_gate := orBool;
     nor_gate := norBool;
+    xor_gate := xorBool;
 }.
 
 
